Safety

spc/Safe.v
@@ -6,13 +6,14 @@ Require Import Skeleton.
 Require Import PCM.
 From Ordinal Require Export Ordinal Arithmetic Inaccessible.
 Require Import Any.
-Require Import IRed.
+Require Import Red IRed.
 
 From ExtLib Require Import
      Core.RelDec
      Structures.Maps
      Data.Map.FMapAList.
 
+Require Import SimGlobal.
 Require Import HoareDef.
 Require Import List.
 
@@ -38,6 +39,23 @@ Section SAFEMODSEM.
       guarantee (stb fn);;;
       trigger (Call fn varg);;;
       tau;; safe_itree.
+
+  Lemma safe_itree_red:
+    safe_itree =
+    break <- trigger (Choose _);;
+    if break: bool
+    then
+      ret <- trigger (Choose _);;
+      guarantee (finalize ret <> None);;;
+                Ret ret
+    else
+      '(fn, varg) <- trigger (Choose _);;
+      guarantee (stb fn);;;
+                trigger (Call fn varg);;;
+                tau;; safe_itree.
+  Proof.
+    eapply itree_eta_eq. ss.
+  Qed.
 
   Definition safe_specbody (fsp: fspec): fspecbody :=
     mk_specbody fsp (fun _ => safe_itree).
@@ -127,6 +145,7 @@ Section LEMMAS.
   Hint Resolve safe_state_mon: paco.
 
   Definition safe_state := paco3 _safe_state bot3.
+  Arguments safe_state [_] _ _.
 
   Variant safe_bind_clo
           (r: forall R, (R -> Prop) -> itree eventE R -> Prop)
@@ -179,15 +198,36 @@ Section LEMMAS.
     eapply safe_bind_clo_wrespectful.
   Qed.
 
-  Definition safe_ret_val: Any.t -> Prop :=
+  Definition safe_retval: Any.t -> Prop :=
     fun x => finalize x <> None.
 
-  Lemma safe_state_no_ub st (SAFE: @safe_state Any.t safe_ret_val st)
+  Lemma safe_state_no_ub st (SAFE: safe_state safe_retval st)
     :
       ~ Beh.of_state L st Tr.ub.
   Proof.
-  Admitted.
+    ii. punfold H0. remember Tr.ub. revert Heqt SAFE.
+    induction H0 using Beh.of_state_ind; ss.
+    { i. inv STEP. des. clarify. eapply IH; auto.
+      punfold SAFE. inv SAFE.
+      { unfold ModSemL.state_sort in SRT. ss. des_ifs. }
+      { eapply step_tau_iff in STEP. des; subst. inv SAFE0; ss. }
+      { eapply step_trigger_choose_iff in STEP. des; subst.
+        specialize (SAFE0 x). inv SAFE0; ss. }
+      { unfold ModSemL.state_sort in SRT. ss. }
+    }
+    { i. punfold SAFE. inv SAFE.
+      { unfold ModSemL.state_sort in SRT. ss. des_ifs. }
+      { unfold ModSemL.state_sort in SRT. ss. }
+      { unfold ModSemL.state_sort in SRT. ss. }
+      { des. inv SAFE0; ss. exploit STEP.
+        { eapply step_trigger_take. }
+        { i. des; clarify. eapply IH; et. }
+      }
+    }
+  Qed.
 End LEMMAS.
+Hint Resolve safe_state_mon: paco.
+Hint Resolve safe_bind_clo_mon: paco.
 
 
 Section SAFETY.
@@ -195,16 +235,84 @@ Section SAFETY.
   Context `{Σ: GRA.t}.
 
   Variable smds: list SafeMod.t.
-
   Variable stb: gname -> Prop.
-  (* Hypothesis stb_sound: *)
-  (*   forall fn (IN: stb fn), In fn (flat_map (fun smd => Safesmd *)
 
   Let mds: list Mod.t := map (SMod.to_src ∘ SafeMod.to_smod stb) smds.
   Hypothesis WF: ModL.wf (Mod.add_list mds).
 
+  Hypothesis stb_sound:
+    forall fn (IN: stb fn),
+      In fn (map fst (ModL.enclose (Mod.add_list mds)).(ModSemL.fnsems)).
+  Hypothesis MAIN:
+    stb "main".
+
+  Ltac ired := try (prw _red_gen 1 0).
+  Ltac step :=
+    unfold assume, guarantee, unwrapN, triggerUB, triggerNB;
+    ired;
+    try (gstep; econs)
+  .
+  Ltac steps := repeat (step; i).
+
+
+  Lemma fnsems_find_safe fn
+    :
+      alist_find fn (ModSemL.fnsems (ModL.enclose (Mod.add_list mds))) = None \/
+      exists mn,
+        alist_find fn (ModSemL.fnsems (ModL.enclose (Mod.add_list mds)))
+        =
+        Some (transl_all (T:=_) mn ∘ fun_to_src (fun _ => SafeModSem.safe_itree stb)).
+  Proof.
+    unfold ModL.enclose, mds.
+    generalize (Sk.sort (ModL.sk (Mod.add_list (map (SMod.to_src ∘ SafeMod.to_smod stb) smds)))).
+    i. rewrite ! Mod.add_list_fnsems.
+    rewrite <- fold_right_app_flat_map. rewrite ! flat_map_map.
+    generalize smds. induction smds0; ss; auto.
+    rewrite ! alist_find_app_o. rewrite ! alist_find_map_snd. uo.
+    change (fun '(fn0, sb) => (fn0: string, fun_to_src (fsb_body sb))) with
+        (map_snd (A:=string) (fun_to_src ∘ fsb_body)).
+    rewrite ! alist_find_map_snd. uo.
+    des_ifs. right. esplits; et.
+  Qed.
+
+  Lemma call_safe:
+    forall md fn arg st
+           (IN: stb fn),
+      paco3 _safe_state bot3 _
+            (fun '(st, retv) => safe_retval retv)
+            (EventsL.interp_Es
+               (ModSemL.prog (ModL.enclose (Mod.add_list mds)))
+               (ModSemL.prog (ModL.enclose (Mod.add_list mds))
+                             (EventsL.Call md fn arg)) st).
+  Proof.
+    ginit. gcofix CIH. i. steps.
+    hexploit stb_sound; et. i.
+    eapply in_map_iff in H0. des. destruct x. clarify.
+    unfold unwrapU. des_ifs.
+    2: { exfalso. eapply alist_find_none in Heq; et. }
+    Local Opaque ModSemL.prog. ss.
+    hexploit (fnsems_find_safe s). i. des; clarify. steps.
+    guclo safe_bind_clo_spec. econs.
+    { instantiate (1:=fun '(st, retv) => safe_retval retv).
+      unfold fun_to_src, body_to_src. generalize st. gcofix CIH0. i.
+      rewrite SafeModSem.safe_itree_red. steps. i. destruct x.
+      { steps. ss. }
+      { steps. destruct x. steps. guclo safe_bind_clo_spec. econs.
+        { gbase. eapply CIH. et. }
+        { i. destruct x0. steps. gbase. eapply CIH0. }
+      }
+    }
+    { i. destruct x. steps. auto. }
+  Qed.
+
   Theorem safe_mods_safe:
     ~ Beh.of_program (ModL.compile (Mod.add_list mds)) Tr.ub.
   Proof.
-  Admitted.
+    eapply safe_state_no_ub. ginit.
+    ss. unfold ModSemL.initial_itr.
+    step. unshelve esplits; et. unfold ITree.map. steps.
+    guclo safe_bind_clo_spec. econs.
+    { gfinal. right. eapply call_safe. auto. }
+    i. destruct x. steps. ss.
+  Qed.
 End SAFETY.
